dw/Custom/List.v
@@ -1,6 +1,48 @@
 From Coq Require Export List.
 Export ListNotations.
 
+Fixpoint take_while {A} (f : A -> bool) (xs : list A) : list A :=
+  match xs with
+  | [] => []
+  | x :: xs =>
+    if f x then
+      x :: take_while f xs
+    else
+      []
+  end.
+
+(* All ways of picking one element in a list apart from the others. *)
+Definition select {X} : list X -> list (X * list X) :=
+  let fix select' pre xs :=
+      match xs with
+      | [] => []
+      | x :: xs' => (x, rev pre ++ xs') :: select' (x :: pre) xs'
+      end in
+  select' [].
+
+Example select_example : select [1;2] = [(1,[2]); (2,[1])].
+Proof. reflexivity. Qed.
+
+Fixpoint filter_opt {A B} (f : A -> option B) (xs : list A) : list B :=
+  match xs with
+  | [] => []
+  | x :: xs =>
+    match f x with
+    | Some y => y :: filter_opt f xs
+    | None => filter_opt f xs
+    end
+  end.
+
+Fixpoint find_opt {A B} (f : A -> option B) (xs : list A) : option B :=
+  match xs with
+  | [] => None
+  | x :: xs =>
+    match f x with
+    | Some y => Some y
+    | None => find_opt f xs
+    end
+  end.
+
 Definition replace_when {A : Type} (f : A -> bool) (new : A) (l : list A) :=
   List.fold_right
     (fun a tail => (if f a then new else a) :: tail)
