dw/Custom/Monad.v
@@ -24,10 +24,8 @@ Notation "f =<< c" := (bind c f)
 Notation "x <- c1 ;; c2" := (bind c1 (fun x => c2))
 (at level 100, c1 at next level, right associativity) : monad_scope.
 
-(*
 Notation "' pat <- c1 ;; c2" := (bind c1 (fun pat => c2))
 (at level 100, pat pattern, c1 at next level, right associativity) : monad_scope.
-*)
 
 Notation "e1 ;; e2" := (_ <- e1%monad ;; e2%monad)%monad
 (at level 100, right associativity) : monad_scope.
