dw/DeepWeb/Spec/Swap_SimpleSpec_Examples.v
@@ -1,0 +1,160 @@
+Require Import Ascii.
+Require Import List.
+Import ListNotations.
+
+Require Import DeepWeb.Lib.Util.
+Require Import DeepWeb.Lib.SimpleSpec.
+Require Import DeepWeb.Spec.Swap_SimpleSpec.
+
+Import EventNotations.
+
+Example trace_example :
+  true = is_trace_of 100 swap_spec_def [
+    0 !;
+    1 !;
+    0 <-- "a";
+    0 <-- "b";
+    0 <-- "c";
+    0 --> "0";
+    0 --> "0";
+    0 --> "0";
+    1 <-- "d";
+    1 <-- "e";
+    1 <-- "f";
+    1 --> "a";
+    1 --> "b";
+    1 --> "c"
+  ].
+Proof. reflexivity. Qed.
+
+Example trace_example2 :
+  false = is_trace_of 100 swap_spec_def [
+    0 !;
+    0 <-- "a";
+    0 <-- "b";
+    0 <-- "c";
+    0 --> "1"
+    (* error: Initial state is 000 *)
+  ].
+Proof. reflexivity. Qed.
+
+Example scrambled_trace_example :
+  is_scrambled_trace_of 1000 swap_spec_def [
+    0 !;
+    1 !;
+    0 <-- "a";
+    0 <-- "b";
+    0 <-- "c";
+    0 --> "0";
+    0 --> "0";
+    0 --> "0";
+    1 <-- "d";
+    1 <-- "e";
+    1 <-- "f";
+    1 --> "a";
+    1 --> "b";
+    1 --> "c"
+  ] = Found [
+    0 !;
+    1 !;
+    0 <-- "a";
+    0 <-- "b";
+    0 <-- "c";
+    0 --> "0";
+    0 --> "0";
+    0 --> "0";
+    1 <-- "d";
+    1 <-- "e";
+    1 <-- "f";
+    1 --> "a";
+    1 --> "b";
+    1 --> "c"
+  ].
+Proof. reflexivity. Qed.
+
+Example scrambled_trace_example_2 :
+  is_scrambled_trace_of 1000 swap_spec_def [
+    0 !;
+    1 !;
+    0 <-- "a";
+    0 <-- "b";
+    0 <-- "c";
+    1 <-- "d";
+    1 <-- "e";
+    1 <-- "f";
+    1 --> "a";
+    1 --> "b";
+    1 --> "c";
+    0 --> "0";
+    0 --> "0";
+    0 --> "0"
+  ] = Found [
+    0 !;
+    1 !;
+    0 <-- "a";
+    0 <-- "b";
+    0 <-- "c";
+    0 --> "0";
+    0 --> "0";
+    0 --> "0";
+    1 <-- "d";
+    1 <-- "e";
+    1 <-- "f";
+    1 --> "a";
+    1 --> "b";
+    1 --> "c"].
+Proof. reflexivity. Qed.
+
+Example scrambled_trace_example_3 :
+  is_scrambled_trace_of 1000 swap_spec_def [
+    0 !;
+    1 !;
+    0 <-- "a";
+    0 <-- "b";
+    0 <-- "c";
+    1 <-- "d";
+    1 <-- "e";
+    1 <-- "f";
+    0 --> "d";
+    0 --> "e";
+    0 --> "f"
+  ] = Found [
+    0 !;
+    1 !;
+    1 <-- "d";
+    1 <-- "e";
+    1 <-- "f";
+    1 --> ?;
+    1 --> ?;
+    1 --> ?;
+    0 <-- "a";
+    0 <-- "b";
+    0 <-- "c";
+    0 --> "d";
+    0 --> "e";
+    0 --> "f"].
+Proof. reflexivity. Qed.
+
+(* This one requires quite a bit of fuel to reject... *)
+Example bad_scrambled_trace_example :
+  is_scrambled_trace_of 2000 swap_spec_def [
+    0 !;
+    1 !;
+    2 !;
+    0 <-- "a";
+    0 <-- "b";
+    0 <-- "c";
+    1 <-- "d";
+    1 <-- "e";
+    1 <-- "f";
+    2 <-- "g";
+    2 <-- "h";
+    2 <-- "i";
+    1 --> "g";
+    1 --> "h";
+    1 --> "i";
+    2 --> "d";
+    2 --> "e";
+    2 --> "f"
+  ] = NotFound.
+Proof. reflexivity. Qed.
