dw/DeepWeb/Test/Rand.v
@@ -1,7 +1,8 @@
 From Coq Require Extraction.
+Require Import DeepWeb.Test.Client.
 
-Parameter flip : unit -> bool.
-Parameter rand : nat -> nat.
+Parameter flip : IO bool.
+Parameter rand : nat -> IO nat.
 
 Extract Constant flip => "Random.bool".
-Extract Constant rand => "Random.int".
+Extract Constant rand => "fun n () -> Random.int n".
